theories/protocol.v
@@ -9,48 +9,146 @@ Require Import Coq.Numbers.DecimalString.
 From Coq Require Import String Ascii List.
 Import ListNotations.
 Require Import   ExtrOcamlString.
+From Coq Require Import String Ascii List Arith.
+Import ListNotations.
+Open Scope string_scope.
 
 Open Scope string_scope.
 
 From Coq Require Import String NArith.
 Open Scope string_scope.
 
-Definition string_of_nat (n : nat) : string :=
-  NilEmpty.string_of_uint (Nat.to_uint n).
+Definition byte := nat.  (* 0..255 *)
+
+From Coq Require Import List String Ascii.
+Import ListNotations.
+
+Definition crlf : list byte := [13;10].
+Definition space : list byte := [32].
+
+(* Definitions *)
+Module Auth.
+  Record t := {
+    username : string;
+    password : string;
+    line : nat;
+    style : string
+  }.
+End Auth.
+
+Module Login.
+  Record t := {
+    username : string;
+    password : string;
+    line : nat
+  }.
+End Login.
+
+Module Connect.
+  Record t := {
+    username : string;
+    password : string;
+    line : nat;
+    destination_ip : string;
+    destination_port : nat
+  }.
+End Connect.
+
+Module Superuser.
+  Record t := {
+    username : string;
+    password : string;
+    line : nat
+  }.
+End Superuser.
+
+Module Logout.
+  Record t := {
+    username : string;
+    password : string;
+    line : nat;
+    reason : string
+  }.
+End Logout.
+
+Module Slipon.
+  Record t := {
+    username : string;
+    password : string;
+    line : nat;
+    slip_address : string
+  }.
+End Slipon.
+
+Module Slipoff.
+  Record t := {
+    username : string;
+    password : string;
+    line : nat;
+    reason : string
+  }.
+End Slipoff.
 
 
-Fixpoint fact (n : nat) : nat :=
-  match n with
-  | O => 1
-  | S n' => n * fact n'
+Inductive request :=
+| Auth (a : Auth.t)
+| Login (l : Login.t)
+| Connect (c : Connect.t)
+| Superuser (s : Superuser.t)
+| Logout (lo : Logout.t)
+| Slipon (so : Slipon.t)
+| Slipoff (sf : Slipoff.t).
+
+
+
+(* Request to byte list *)
+
+Class Serializable (A : Type) := {
+  encode : A -> list byte
+}.
+
+Instance nat_serializable : Serializable nat := {
+  encode s := [45;56]
+}.
+
+Instance string_serializable : Serializable string := {
+  encode s := [78;54] (*List.map (fun c => Nat.of_ascii c) (list_ascii_of_string s)*)
+}.
+
+Fixpoint encode_fields (ll : list (list byte)) : list byte :=
+  match ll with
+  | [] => []
+  | [x] => x           (* last element: no trailing space *)
+  | x :: xs => x ++ space ++ encode_fields xs
+  end.
+
+(* Definition encode_record {A} `{Serializable A} (fields : list A) : list byte :=
+  encode_fields fields ++ crlf.  CRLF *)
+
+Definition encode_variant (tag : byte) (fields : list (list byte)) : list byte :=
+  [tag] ++ encode_fields fields ++ crlf.
+
+
+Definition encode_request_auto (r : request) : list byte :=
+  match r with
+  | Auth a      => encode_variant 0 [encode (Auth.username a); encode (Auth.password a); encode (Auth.line a); encode (Auth.style a)]
+  | Login l     => encode_variant 1 [encode (Login.username l); encode (Login.password l); encode (Login.line l)]
+  | Connect c   => encode_variant 2 [encode (Connect.username c); encode (Connect.password c); encode (Connect.line c); encode (Connect.destination_ip c); encode (Connect.destination_port c)]
+  | Superuser s => encode_variant 3 [encode (Superuser.username s); encode (Superuser.password s); encode (Superuser.line s)]
+  | Logout lo   => encode_variant 4 [encode (Logout.username lo); encode (Logout.password lo); encode (Logout.line lo); encode (Logout.reason lo)]
+  | Slipon so   => encode_variant 5 [encode (Slipon.username so); encode (Slipon.password so); encode (Slipon.line so); encode (Slipon.slip_address so)]
+  | Slipoff sf  => encode_variant 6 [encode (Slipoff.username sf); encode (Slipoff.password sf); encode (Slipoff.line sf); encode (Slipoff.reason sf)]
   end.
 
 
 
-
-Record auth_request := {
-  version : nat;
-  req_type : string;
-  username : string;
-  password : string;
-  line     : nat
-}.
-
-
-Definition make_package (req : auth_request) : list string :=
-  [ string_of_nat req.(version) ++ " " ++ req.(req_type) ;
-    req.(username) ;
-    req.(password) ;
-    string_of_nat req.(line) ].
+(* byte to request *)
 
 
 
-
-(* Force string to be extracted as OCaml string *)
-(* Extract Inductive string => "string" [ """" "(^)" ].
-Extract Constant append => "(^)".  *)
-
+(* Extraction stuff *)
 Require Extraction.
+
 Set Extraction Output Directory "../../theories".
 Extraction Language OCaml.
-Extraction "tacacs_extracted.ml" fact auth_request make_package. 
+Extraction "tacacs_extracted.ml" request encode_request_auto. 
